Veir.lean
@@ -9,6 +9,7 @@ import Veir.Rewriter.InlineBlock
 import Veir.Rewriter.WfRewriter
 import Veir.Printer
 import Veir.PatternRewriter.Basic
+import Veir.Fold.Semantics
 import Veir.Passes.RISCVCombines.Proofs
 import Veir.Benchmarks
 import Veir.Parser.Lexer
